{-
  Here the Automata and its operations are defined according to:
    The Theory of Parsing, Translation and Compiling (Vol. 1 : Parsing)
    Section 2.2: Regular sets, their generators, and their recognizers
      by Alfred V. Aho and Jeffery D. Ullman

  Steven Cheung 2015.
  Version 27-02-2016
-}
open import Util
module eNFA (Σ : Set)(dec : DecEq Σ) where

open import Data.List hiding (any ; all) 
open import Relation.Binary.PropositionalEquality
open import Data.Product hiding (Σ)
open import Data.Nat

open import Subset.DecidableSubset
  renaming (_∈?_ to _∈ᵈ?_ ; _∈_ to _∈ᵈ_ ; _∉_ to _∉ᵈ_ ; Ø to Øᵈ ; _⋃_ to _⋃ᵈ_ ; _⋂_ to _⋂ᵈ_ ; ⟦_⟧ to ⟦_⟧ᵈ
                 ; _≈_ to _≈ᵈ_ ; _⊆_ to _⊆ᵈ_ ; _⊇_ to _⊇ᵈ_ ; ≈-refl to ≈ᵈ-refl ; ≈-trans to ≈ᵈ-trans ; ≈-sym to ≈ᵈ-sym)
open import Data.Vec
open import Data.Vec.Membership.Propositional renaming  (_∈_ to _∈ⱽ_                ) hiding (_∉_      )
open import Subset.VectorRep renaming (_∈?_ to _∈ⱽ?_)
open import Language Σ dec

-- Nondeterministic finite automata with ε-step
-- section 2.2.3: Finite Automata
record ε-NFA : Set₁ where
  field
    Q      : Set
    δ      : Q → Σᵉ → DecSubset Q
    q₀     : Q
    F      : DecSubset Q
    ∀qEq   : ∀ q → q ∈ᵈ δ q E
    Q?     : DecEq Q
    ∣Q∣-1  : ℕ
    It     : Vec Q (suc ∣Q∣-1)
    ∀q∈It  : (q : Q) → (q ∈ⱽ It)
    unique : Unique It

-- section 2.2.3: Finite Automata
module ε-NFA-Operations (N : ε-NFA) where
  open ε-NFA N

  -- a move from (q , aw) to (q' , w)
  infix 7 _⊢_
  _⊢_ : (Q × Σᵉ × Σᵉ*) → (Q × Σᵉ*) → Set
  (q , aᵉ , wᵉ) ⊢ (q' , wᵉ') = wᵉ ≡ wᵉ' × q' ∈ᵈ δ q aᵉ

  -- k moves from (q , w) to (q' , w')
  infix 7 _⊢ᵏ_─_
  _⊢ᵏ_─_ : (Q × Σᵉ*) → ℕ → (Q × Σᵉ*) → Set
  (q , wᵉ) ⊢ᵏ zero    ─ (q' , wᵉ')
    = q ≡ q' × wᵉ ≡ wᵉ'
  (q , wᵉ) ⊢ᵏ (suc n) ─ (q' , wᵉ')
    = Σ[ p ∈ Q ] Σ[ aᵉ ∈ Σᵉ ] Σ[ uᵉ ∈ Σᵉ* ]
      ( wᵉ ≡ aᵉ ∷ uᵉ × (q , aᵉ , uᵉ) ⊢ (p , uᵉ) × (p , uᵉ) ⊢ᵏ n ─ (q' , wᵉ') )
  
  -- transitive closure of ⊢
  infix 7 _⊢*_
  _⊢*_ : (Q × Σᵉ*) → (Q × Σᵉ*) → Set
  (q , wᵉ) ⊢* (q' , wᵉ') = Σ[ n ∈ ℕ ] (q , wᵉ) ⊢ᵏ n ─ (q' , wᵉ')


-- Language denoted by a ε-NFA
-- section 2.2.3: Finite Automata
-- L(nfa) = { w | ∃wᵉ∈Σᵉ*. w ≡ toΣ* wᵉ ∧ ∃q∈F. (q₀ , wᵉ) ⊢* (q , []) }
Lᵉᴺ : ε-NFA → Language
Lᵉᴺ nfa = λ w → Σ[ wᵉ ∈ Σᵉ* ] (w ≡ toΣ* wᵉ × ( Σ[ q ∈ Q ] ( q ∈ᵈ F × (q₀ , wᵉ) ⊢* (q , [])) ))
  where
    open ε-NFA nfa
    open ε-NFA-Operations nfa



module ε-NFA-Properties (N : ε-NFA) where

  open ε-NFA N
  open ε-NFA-Operations N

  -- alternative definition of ⊢ᵏ
  infix 7 _⊢ᵏ₂_─_
  _⊢ᵏ₂_─_ : (Q × Σᵉ*) → ℕ → (Q × Σᵉ*) → Set
  (q , wᵉ) ⊢ᵏ₂ zero ─ (q' , wᵉ')
    = (q , wᵉ) ⊢ᵏ zero ─ (q' , wᵉ')
  (q , wᵉ) ⊢ᵏ₂ (suc n) ─ (q' , wᵉ')
    = Σ[ p ∈ Q ] Σ[ aᵉ ∈ Σᵉ ]
      ( (q , wᵉ) ⊢ᵏ n ─ (p , aᵉ ∷ wᵉ') × (p , aᵉ , wᵉ') ⊢ (q' , wᵉ') )
  
  -- ⊢ᵏ ⇔ ⊢ᵏ₂
  -- actual proofs are in the bottom
  ⊢ᵏ⇔⊢ᵏ₂ : ∀ {q wᵉ n q' wᵉ'}
           → (q , wᵉ) ⊢ᵏ n ─ (q' , wᵉ') ⇔ (q , wᵉ) ⊢ᵏ₂ n ─ (q' , wᵉ')
  
  
  -- alternative definition of ⊢*
  infix 7 _⊢*₂_
  _⊢*₂_ : (Q × Σᵉ*) → (Q × Σᵉ*) → Set
  (q , wᵉ) ⊢*₂ (q' , wᵉ')
    = Σ[ n ∈ ℕ ] Σ[ m ∈ ℕ ] Σ[ p ∈ Q ] Σ[ uᵉ ∈ Σᵉ* ]
      ((q , wᵉ) ⊢ᵏ n ─ (p , uᵉ) × (p , uᵉ) ⊢ᵏ m ─ (q' , wᵉ'))
  
  -- ⊢* ⇔ ⊢*₂
  -- actual proofs are in the bottom
  ⊢*⇔⊢*₂ : ∀ {q wᵉ q' wᵉ'}
             → (q , wᵉ) ⊢* (q' , wᵉ') ⇔ (q , wᵉ) ⊢*₂ (q' , wᵉ')
  
  
  {- below are the proofs of ⊢ᵏ ⇔ ⊢ᵏ₂ -}
  find-p : ∀ q wᵉ n q' wᵉ'
         → (q , wᵉ) ⊢ᵏ suc n ─ (q' , wᵉ')
         → Q
  find-p q ._ zero    .p  .uᵉ  (p , a , uᵉ , refl , prf₁ , (refl , refl))
    = q
  find-p q ._ (suc n)  q'  wᵉ' (p , a , uᵉ , refl , prf₁ , prf₂)
    = find-p p uᵉ n q' wᵉ' prf₂
  
  find-a : ∀ q wᵉ n q' wᵉ'
           → (q , wᵉ) ⊢ᵏ suc n ─ (q' , wᵉ')
           → Σᵉ
  find-a q ._ zero    .p  .uᵉ  (p , aᵉ , uᵉ , refl , prf₁ , (refl , refl))
    = aᵉ
  find-a q ._ (suc n)  q'  wᵉ' (p , aᵉ , uᵉ , refl , prf₁ , prf₂)
    = find-a p uᵉ n q' wᵉ' prf₂
  
  ⊢ᵏ₂-lem₈ : ∀ q wᵉ n q' wᵉ'
             → (prf : (q , wᵉ) ⊢ᵏ suc n ─ (q' , wᵉ'))
             → Σ[ p ∈ Q ] Σ[ a ∈ Σᵉ ]
               (p ≡ find-p q wᵉ n q' wᵉ' prf
                 × a ≡ find-a q wᵉ n q' wᵉ' prf
                 × (p , a , wᵉ') ⊢ (q' , wᵉ'))
  ⊢ᵏ₂-lem₈ q ._ zero    .p  .uᵉ  (p , a , uᵉ , refl , prf₁ , (refl , refl))
    = q , a , refl , refl , prf₁
  ⊢ᵏ₂-lem₈ q ._ (suc n)  q'  wᵉ' (p , a , uᵉ , refl , prf₁ , prf₂)
    = ⊢ᵏ₂-lem₈ p uᵉ n q' wᵉ' prf₂
  
  ⊢ᵏ₂-lem₇ : ∀ q wᵉ n q' wᵉ' p a
             → (prf : (q , wᵉ) ⊢ᵏ suc n ─ (q' , wᵉ'))
             → p ≡ find-p q wᵉ n q' wᵉ' prf
             → a ≡ find-a q wᵉ n q' wᵉ' prf
             → (q , wᵉ) ⊢ᵏ n ─ (p , a ∷ wᵉ')
  ⊢ᵏ₂-lem₇ q ._ zero    .p' .uᵉ  p a (p' , a' , uᵉ , refl , prf₁ , (refl , refl)) p≡q a≡a'
    = sym p≡q , cong (λ a → a ∷ uᵉ) (sym a≡a')
  ⊢ᵏ₂-lem₇ q ._ (suc n)  q'  wᵉ' p a (p' , a' , uᵉ , refl , prf₁ ,          prf₂) p≡p a≡a
    = p' , a' , uᵉ , refl , prf₁ , ⊢ᵏ₂-lem₇ p' uᵉ n q' wᵉ' p a prf₂ p≡p a≡a
  
  ⊢ᵏ₂-lem₆ : ∀ q wᵉ n q' wᵉ'
             → (prf : (q , wᵉ) ⊢ᵏ suc n ─ (q' , wᵉ'))
             → Σ[ p ∈ Q ] Σ[ a ∈ Σᵉ ]
               (p ≡ find-p q wᵉ n q' wᵉ' prf
                 × a ≡ find-a q wᵉ n q' wᵉ' prf
                 × (q , wᵉ) ⊢ᵏ n ─ (p , a ∷ wᵉ'))
  ⊢ᵏ₂-lem₆ q wᵉ n q' wᵉ' prf
    = p , a , refl , refl , ⊢ᵏ₂-lem₇ q wᵉ n q' wᵉ' p a prf refl refl
    where
      p : Q
      p = find-p q wᵉ n q' wᵉ' prf
      a : Σᵉ
      a = find-a q wᵉ n q' wᵉ' prf
  
  ⊢ᵏ₂-lem₅ : ∀ q wᵉ n q' wᵉ'
             → (prf : (q , wᵉ) ⊢ᵏ suc n ─ (q' , wᵉ'))
             → Σ[ p ∈ Q ] Σ[ a ∈ Σᵉ ]
               (p ≡ find-p q wᵉ n q' wᵉ' prf
                 × a ≡ find-a q wᵉ n q' wᵉ' prf
                 × (q , wᵉ) ⊢ᵏ n ─ (p , a ∷ wᵉ')
                 × (p , a , wᵉ') ⊢ (q' , wᵉ'))
  ⊢ᵏ₂-lem₅ q wᵉ n q' wᵉ' prf with ⊢ᵏ₂-lem₆ q wᵉ n q' wᵉ' prf | ⊢ᵏ₂-lem₈ q wᵉ n q' wᵉ' prf
  ... | p₁ , a₁ , p₁≡p , a₁≡a , prf₁ |  p₂ , a₂ , p₂≡p , a₂≡a , prf₂
    = p₁ , a₁ , p₁≡p , a₁≡a , prf₁ , prf₂''
    where
      prf₂' : (p₁ , a₂ , wᵉ') ⊢ (q' , wᵉ')
      prf₂' = subst (λ p₁ → (p₁ , a₂ , wᵉ') ⊢ (q' , wᵉ')) (trans p₂≡p (sym p₁≡p)) prf₂
      prf₂'' : (p₁ , a₁ , wᵉ') ⊢ (q' , wᵉ')
      prf₂'' = subst (λ a₁ → (p₁ , a₁ , wᵉ') ⊢ (q' , wᵉ')) (trans a₂≡a (sym a₁≡a)) prf₂'
    
  ⊢ᵏ₂-lem₄ : ∀ q wᵉ n q' wᵉ'
             → (q , wᵉ) ⊢ᵏ suc n ─ (q' , wᵉ')
             → (q , wᵉ) ⊢ᵏ₂ suc n ─ (q' , wᵉ')
  ⊢ᵏ₂-lem₄ q wᵉ n q' wᵉ' prf with ⊢ᵏ₂-lem₅ q wᵉ n q' wᵉ' prf
  ... | p' , a' , p≡p' , a≡a' , prf₁ = p , a , prf₁''
    where
      p : Q
      p = find-p q wᵉ n q' wᵉ' prf
      a : Σᵉ
      a = find-a q wᵉ n q' wᵉ' prf
      prf₁' : (q , wᵉ) ⊢ᵏ n ─ (p , a' ∷ wᵉ') × (p , a' , wᵉ') ⊢ (q' , wᵉ')
      prf₁' = subst (λ p → (q , wᵉ) ⊢ᵏ n ─ (p , a' ∷ wᵉ') × (p , a' , wᵉ') ⊢ (q' , wᵉ')) p≡p' prf₁
      prf₁'' : (q , wᵉ) ⊢ᵏ n ─ (p , a ∷ wᵉ') × (p , a , wᵉ') ⊢ (q' , wᵉ')
      prf₁'' = subst (λ a → (q , wᵉ) ⊢ᵏ n ─ (p , a ∷ wᵉ') × (p , a , wᵉ') ⊢ (q' , wᵉ')) a≡a' prf₁'
  
  ⊢ᵏ₂-lem₉ : ∀ {q wᵉ n p a q' wᵉ'}
             → (q , wᵉ) ⊢ᵏ n ─ (p , a ∷ wᵉ')
             → (p , a , wᵉ') ⊢ (q' , wᵉ')
             → (q , wᵉ) ⊢ᵏ suc n ─ (q' , wᵉ')
  ⊢ᵏ₂-lem₉ {.p} {._} {zero}  {p} {a} {q'} {wᵉ'} (refl , refl) prf = q' , a , wᵉ' , refl , prf , (refl , refl)
  ⊢ᵏ₂-lem₉ {q}  {._} {suc n} {p} {a} {q'} {wᵉ'} (p₁ , a₁ , u₁ , refl , prf₁ , prf₂) prf₃
    = p₁ , a₁ , u₁ , refl , prf₁ , ⊢ᵏ₂-lem₉ {p₁} {u₁} {n} {p} {a} {q'} {wᵉ'} prf₂ prf₃
  
  ⊢ᵏ₂-lem₃ : ∀ {q wᵉ n q' wᵉ'}
             → (q , wᵉ) ⊢ᵏ₂ n ─ (q' , wᵉ')
             → (q , wᵉ) ⊢ᵏ n ─ (q' , wᵉ')
  ⊢ᵏ₂-lem₃ {q} {wᵉ} {zero}  {.q} {.wᵉ} (refl , refl) = refl , refl
  ⊢ᵏ₂-lem₃ {q} {wᵉ} {suc n} {q'} {wᵉ'} (p , a , prf₁ , prf₂)
    = ⊢ᵏ₂-lem₉ {q} {wᵉ} {n} {p} {a} {q'} {wᵉ'} prf₁ prf₂
  
  ⊢ᵏ₂-lem₂ : ∀ {q wᵉ n q' wᵉ'}
             → (q , wᵉ) ⊢ᵏ n ─ (q' , wᵉ')
             → (q , wᵉ) ⊢ᵏ₂ n ─ (q' , wᵉ')
  ⊢ᵏ₂-lem₂ {q} {wᵉ} {zero}  {.q} {.wᵉ} (refl , refl)
    = refl , refl
  ⊢ᵏ₂-lem₂ {q} {wᵉ} {suc n} {q'} {wᵉ'} prf
    = ⊢ᵏ₂-lem₄ q wᵉ n q' wᵉ' prf
                             
  ⊢ᵏ⇔⊢ᵏ₂ {q} {wᵉ} {n} {q'} {wᵉ'}
    = ⊢ᵏ₂-lem₂ {q} {wᵉ} {n} {q'} {wᵉ'} , ⊢ᵏ₂-lem₃ {q} {wᵉ} {n} {q'} {wᵉ'}
  {- above are the proofs of ⊢ᵏ ⇔ ⊢ᵏ₂ -}
  
  {- below are the proofs of ⊢* ⇔ ⊢*₂ -}
  ⊢*-lem₄ : ∀ q wᵉ n p uᵉ m q' wᵉ'
            → (q , wᵉ) ⊢ᵏ n ─ (p , uᵉ)
            → (p , uᵉ) ⊢ᵏ m ─ (q' , wᵉ')
            → (q , wᵉ) ⊢ᵏ n + m ─ (q' , wᵉ')
  ⊢*-lem₄ .p wᵉ zero     p .wᵉ m q'  wᵉ' (refl , refl) prf
    = prf
  ⊢*-lem₄  q wᵉ (suc n)  p  uᵉ m q'  wᵉ' (r , a , vᵉ , prf₁ , prf₂ , prf₃) prf₄
    = r , a , vᵉ , prf₁ , prf₂ , ⊢*-lem₄ r vᵉ n p uᵉ m q' wᵉ' prf₃ prf₄
                                                                   
  ⊢*-lem₃ : ∀ {q wᵉ q' wᵉ'}
            → (q , wᵉ) ⊢*  (q' , wᵉ')
            → (q , wᵉ) ⊢*₂ (q' , wᵉ')
  ⊢*-lem₃ {q} {wᵉ} {q'} {wᵉ'} (n , prf)
    = n , zero , q' , wᵉ' , prf , (refl , refl)
  
  ⊢*-lem₂ : ∀ {q wᵉ q' wᵉ'}
            → (q , wᵉ) ⊢*₂ (q' , wᵉ')
            → (q , wᵉ) ⊢*  (q' , wᵉ')
  ⊢*-lem₂ {q} {wᵉ} {q'} {wᵉ'} (n , m , p , uᵉ , prf₁ , prf₂)
    = n + m , ⊢*-lem₄ q wᵉ n p uᵉ m q' wᵉ' prf₁ prf₂
  
  ⊢*⇔⊢*₂ = ⊢*-lem₃ , ⊢*-lem₂
  {- above are the proofs of ⊢* ⇔ ⊢*₂ -}
     
